add more proof

TransVal/Crash.v
@@ -1,8 +1,13 @@
 Require Import IL StateType.
 
 Inductive Crash : F.state -> F.state -> Prop :=
+|CrashReturn L E e:
+exp_eval E e = None
+-> state_result (L,E, stmtReturn e) = None
+-> Crash (L,E,stmtReturn e) (L, E, stmtReturn e)
 |CrashBase L E s :
- normal2 F.step (L, E, s)
+(forall e, s <> stmtReturn e)
+->  normal2 F.step (L, E, s)
 -> state_result (L,E,s) = None
 -> Crash (L, E,s) (L,E,s)
 |CrashStep sigma sigma' sigma'' a:
